taking G out of context

src/coq_formalism/reduce.v
@@ -16,19 +16,19 @@ Section Reducer.
 
     Context {measurement : Type}.
     Context {corruption : Type}.
-    Context {G : attackgraph measurement corruption}.
+    (* Context {G : attackgraph measurement corruption}.*)
 
     (* Labels and States must have decidable equality *)
     Hypothesis eqDec_measurement : forall (x y : measurement), {x = y} + {x <> y}.
     Hypothesis eqDec_corruption : forall (x y : corruption), {x = y} + {x <> y}.
-    Hypothesis eqDec_state : forall (x y : G.(state _ _)), {x = y} + {x <> y}.
+    Hypothesis eqDec_state :  forall (G : attackgraph measurement corruption) (x y : G.(state _ _)), {x = y} + {x <> y}.
 
     (* steps are equivalent or not equivalent *)
-    Lemma eqDec_step : forall (x y : G.(state _ _) * G.(state _ _)), {x = y} + {x <> y}.
+    Lemma eqDec_step : forall (G : attackgraph measurement corruption) (x y : (G.(state _ _) * G.(state _ _))), {x = y} + {x <> y}.
     Proof.
-        intros x y;
+        intros G x y;
         destruct x as [stx stx']; destruct y as [sty sty'].
-        destruct eqDec_state with (x:=stx) (y:=sty).
+        destruct eqDec_state with (G := G) (x:=stx) (y:=sty).
         + destruct eqDec_state with (x:=stx') (y:=sty').
         ++ subst. left. eauto.  
         ++ right. intros contra. rewrite pair_equal_spec in contra. destruct contra. contradiction.
@@ -38,64 +38,64 @@ Section Reducer.
     Qed.
 
     (* list of steps are decidably equal *)
-    Lemma eqDec_list_steps: forall (x y : list (G.(state _ _) * G.(state _ _))), {x = y} + {x <> y}.
+    Lemma eqDec_list_steps: forall `{G : attackgraph measurement corruption} (x y : list (G.(state _ _) * G.(state _ _))), {x = y} + {x <> y}.
     Proof.
-        apply list_eq_dec. apply eqDec_step.
+        intros G. apply list_eq_dec. apply eqDec_step.
     Qed.
 
-    Fixpoint replace_measurement_incomplete (Steps : list (G.(state _ _) * G.(state _ _))) (st st' : (G.(state _ _))) : 
+    Fixpoint replace_measurement_incomplete {G: attackgraph measurement corruption} (Steps : list (G.(state _ _) * G.(state _ _))) (st st' : (G.(state _ _))) : 
                                  list (G.(state _ _) * G.(state _ _)) := 
         match Steps with 
-        | (st1, st2) :: Steps' => if (eqDec_state st st2)
+        | (st1, st2) :: Steps' => if (eqDec_state G st st2)
                                   then (st1, st') :: replace_measurement_incomplete Steps' st st' 
                                   else (st1, st2) :: replace_measurement_incomplete Steps' st st'
         | nil => Steps 
         end. 
 
     (* Replace all occurences of st by st' in Steps *)
-    Fixpoint replace_measurement (Steps : list (G.(state _ _) * G.(state _ _))) 
+    Fixpoint replace_measurement {G : attackgraph measurement corruption} (Steps : list (G.(state _ _) * G.(state _ _))) 
     (st st' : G.(state _ _)) : 
     list (G.(state _ _) * G.(state _ _)) :=
     match Steps with
     | (st1, st2) :: Steps' => 
-        if (eqDec_state st1 st)
-        then if (eqDec_state st2 st)
+        if (eqDec_state G st1 st)
+        then if (eqDec_state G st2 st)
             then (st', st') :: replace_measurement Steps' st st'
             else (st', st2) :: replace_measurement Steps' st st'
-        else if (eqDec_state st2 st)
+        else if (eqDec_state G st2 st)
             then (st1, st') :: replace_measurement Steps' st st'
             else (st1, st2) :: replace_measurement Steps' st st'
     | nil => Steps
     end.
-
-    Lemma replace_measurement_same : forall Steps st st', 
-    replace_measurement_incomplete Steps st st' = replace_measurement Steps st st'.
-    Proof.
-        intros. simpl. induction Steps. 
-        + eauto.
-        + simpl. rewrite IHSteps. simpl.
-        (* although I think replace_measurement_incomplete is sufficient... I can't prove they are the same. *)
-    Abort.
-
-    (* Inductively defined replace_measurement *)
-    Inductive replace_measurement' (Steps : list (G.(state _ _) * G.(state _ _))) (st st' : G.(state _ _)) : list (G.(state _ _) * G.(state _ _)) -> Prop := 
-    | TheEnd : replace_measurement' Steps st st' nil.
     
-    Fixpoint find_measurement (AllSteps Steps : list (G.(state _ _) * G.(state _ _))) : 
-                                list (G.(state _ _) * G.(state _ _)) := 
+    Print eqDec_step.
+    Print remove.
+
+    Fixpoint find_measurement {G : attackgraph measurement corruption} (AllSteps Steps : list (G.(state _ _) * G.(state _ _))) :  list (G.(state _ _) * G.(state _ _)) := 
     match Steps with 
     | (st, st') :: Steps' => match (G.(label _ _) st) with 
                              | inr c1 => find_measurement AllSteps Steps' 
                              | inl m1 => match (G.(label _ _) st') with 
                                          (* if both m1 and m2 are measurement events then you can replace them *)
-                                         | inl m2 => replace_measurement (remove eqDec_step (st, st') AllSteps) st st' 
+                                         | inl m2 => replace_measurement (remove (eqDec_step _ ) (st, st') AllSteps) st st' 
                                          | _ => find_measurement AllSteps Steps'
                                          end
                              end
     | nil => AllSteps
     end.
-        
-    Definition reduce1 (Steps : list (G.(state _ _) * G.(state _ _))) : list (G.(state _ _) * G.(state _ _)) :=
+
+    (* finding measurement x in x should return x? *)
+    Lemma find_measurement_helper : forall (G : attackgraph measurement corruption) (x : list(G.(state _ _) * G.(state _ _))), find_measurement x x = x.
+    Proof.
+        intros. induction x.
+        + auto.
+        + (* simpl. destruct a. destruct (G.(label _ _) s) eqn:l_a .
+        ++ destruct (G.(label _ _) s0) eqn:l_a2.
+        +++ simpl in *. destruct ((eqDec_step G) (s, s0) (s, s0)).
+        ++++ simpl. unfold remove. unfold replace_measurement.*)
+    Abort.
+
+    Definition reduce1 `{G : attackgraph measurement corruption} (Steps : list (G.(state _ _) * G.(state _ _))) : list (G.(state _ _) * G.(state _ _)) :=
     find_measurement Steps Steps.
 
     (* We cannot define a recursive fixpoint because of 
@@ -107,16 +107,50 @@ Section Reducer.
      * then the graph cannot be further reduced. If reduce1
      * does not return itself, then the reduction call is
      * recursed. *)
-    Inductive reducer : list (G.(state _ _) * G.(state _ _)) -> list (G.(state _ _) * G.(state _ _)) -> Prop :=
+    Inductive reducer {G : attackgraph measurement corruption} : list (G.(state _ _) * G.(state _ _)) -> list (G.(state _ _) * G.(state _ _)) -> Prop :=
     | reduce_done : forall x, reduce1 x = x -> reducer x x
     | reduce_more : forall x y, reduce1 x <> x -> reducer (reduce1 x) y -> reducer x y.  
 
-    Theorem  reducer_trans : forall x y, reducer x y -> forall z, reducer y z -> reducer x z.
+    Definition reduce_graph g1 := reducer (g1.(steps _ _)).  
+
+    (* a graph may always reduce to itself *)
+    Theorem reducer_refl : forall (G : attackgraph measurement corruption) (x : list(G.(state _ _) * G.(state _ _))), reducer x x.
     Proof.
-        intros x y Hxy. induction Hxy.
+        intros.
+        induction x.
+        + econstructor. unfold reduce1. eauto.
+        + apply reduce_done. unfold reduce1. 
+    Abort.
+    (* Proof is hard and might not be possible? *)
+
+
+    (* if a graph reduces from x to y and then y to z then you can say x reduces to z *)
+    Theorem  reducer_trans : forall (G : attackgraph measurement corruption) (x : list(G.(state _ _) * G.(state _ _))) (y : list(G.(state _ _) * G.(state _ _))) , reducer x y -> forall (z : list(G.(state _ _) * G.(state _ _))) , reducer y z -> reducer x z.
+    Proof.
+        intros G x y Hxy. induction Hxy.
         + eauto.
         + intros. apply reduce_more; eauto.
     Qed.
-    (* want reducer to be more similiar to equivalence *)  
+
+    (* prove reducer is total... ie it holds for any two lists *)
+
+    Print eqDec_step.
+    Print reducer. 
+
+    Theorem  reducer_total : forall (G : attackgraph measurement corruption) (x : list(G.(state _ _) * G.(state _ _))) (y : list(G.(state _ _) * G.(state _ _))), reducer x y.
+    Proof.
+        intros. induction x.
+        + econstructor. eauto. 
+        pose proof list_eq_dec.
+        pose proof (eqDec_step G).
+        induction X with (A := (state measurement corruption G * state measurement corruption G )) (l := x) (l' := y).
+        intuition.
+
+        
+    Qed.
+    
+
+
+
 
 End Reducer.
